heaps memory definition

KLR/Semantics/Memory.lean
@@ -9,28 +9,62 @@ import KLR.Core.Basic
 import KLR.Util
 import Iris.Instances.heProp
 
+/-- A multiaffine equation describing an access into a free coordinate of an Address -/
+structure AffineMap where
+  free_offset : Int
+  free_strides : List Int
+  par_offset : Int
+  par_stride : Int
+  deriving Repr, BEq
+
+def AffineMap.par (a : AffineMap) (i : Int) : Int :=
+  a.par_offset + a.par_stride * i
+
+def AffineMap.free (a : AffineMap) (i : List Int) : Int :=
+  a.free_offset + List.dot a.free_strides i
+
+def AffineMap.is_trivial (a : AffineMap) : Prop :=
+  a.free_offset = 0 ∧
+  a.par_offset = 0 ∧
+  a.par_stride = 1 ∧
+  a.free_strides = a.free_strides.map (fun _ => 1)
+
 namespace KLR.Core
 
 /-- A LocalStore represents an unboudned 2D region of memory. -/
 structure LocalStore (α : Type _) where
   elems : Nat × Nat → Option α
 
-instance : Inhabited (LocalStore α) where default :=
-  ⟨ fun _ => .none ⟩
+instance : Heap (LocalStore α) (Nat × Nat) α where
+  get s c := s.elems c
+  set s n v := { elems n' := if n = n' then v else s.elems n' }
+  empty := { elems _ := none }
+  hmap f s := { elems n := s.elems n |>.bind (f n) }
+  merge op x y := { elems n := Option.merge op (x.elems n) (y.elems n) }
+  get_set_eq := by simp_all
+  get_set_ne := by simp_all
+  get_empty  := by simp_all
+  get_hmap   := by simp_all
+  get_merge  := by simp_all
 
-@[simp] def LocalStore.get (s : LocalStore α) (c : Nat × Nat) : Option α := s.elems c
+instance {α β} : HasHHMap (LocalStore α) (LocalStore β) (Nat × Nat) α β where
+  hhmap f s := ⟨fun i => Store.get s i |>.bind (f i)⟩
+  hhmap_get {t k} f := by simp [Store.get]
 
-@[simp] def LocalStore.set (s : LocalStore α) (c : Nat × Nat) (v : Option α) :=
-  { s with elems c' := if c == c' then v else s.elems c }
+instance : Inhabited (LocalStore α) where default := ⟨ fun _ => .none ⟩
 
-/-- A PhyStore represents an bounded 2D region of memory, encoeded as a LocalStore with
-an additional inbounds predicate. -/
-structure PhyStore (α : Type _) extends LocalStore α where
+/-
+structure PhyStoreSpec where
   pmax : Nat
   fmax : Nat
 
-@[simp] def PhyStore.inbounds (s : PhyStore α) (c : Nat × Nat) : Bool :=
-  c.1 < s.pmax && c.2 < s.fmax
+@[simp] def PhyStoreSpec.inbounds (s : PhyStoreSpec) (c : Nat × Nat) : Prop :=
+  c.1 < s.pmax ∧ c.2 < s.fmax
+
+structure PhyStoreIndex (s : PhyStoreSpec) where
+  index : Nat × Nat
+  wf : s.inbounds index
+-/
 
 /-
 A model of NeuronCore memory banks.
@@ -55,55 +89,210 @@ and equivalences to programs involving realistic allocation modes need only be d
 at the peripheries.
 -/
 
-abbrev UnboundedBank (α : Type _) := Array (LocalStore α)
-abbrev UnboundedBank.inbounds (d : UnboundedBank α) (i : Nat) : Bool := i < d.size
-abbrev UnboundedBank.get (d : UnboundedBank α) (i : Nat) : LocalStore α := d[i]!
-abbrev UnboundedBank.set (d : UnboundedBank α) (i : Nat) (v : LocalStore α → LocalStore α) : UnboundedBank α :=
-  d.mapIdx (fun i' s => if i' == i then v s else s)
-abbrev UnboundedBank.push (d : UnboundedBank α) (l : LocalStore α) : UnboundedBank α :=
-  Array.push d l
 
-structure DualMemory (α : Type _) where
-  bounded : PhyStore α
-  unbounded : UnboundedBank α
+structure TensorBank (α : Type _) where
+  bank : Nat → Option (LocalStore α)
+  next_fresh : Nat
 
-inductive DualMemoryStoreIndex
-| in_bounded
-| in_unbounded (i : Nat)
-  deriving Repr, BEq
+/-- Well-formedness of a TensorBank. -/
+@[simp] def TensorBank.wf (c : TensorBank α) : Prop :=
+  ∀ n, c.next_fresh ≤ n → c.bank n = none
 
-def DualMemory.in_memory {α} (d : DualMemory α) : DualMemoryStoreIndex → Prop
-| .in_bounded => True
-| .in_unbounded i => i < d.unbounded.size
+instance : UnboundedHeap (TensorBank α) Nat (LocalStore α) where
+  get b n := b.bank n
+  set b n v := { bank := fun n' => if n' = n then v else b.bank n', next_fresh := max b.next_fresh n+1 }
+  empty := { bank := fun _ => none, next_fresh := 0 }
+  hmap f b := { bank n := (b.bank n).bind (f n), next_fresh := b.next_fresh}
+  merge op x y := { bank n := Option.merge op (x.bank n) (y.bank n), next_fresh := max x.next_fresh y.next_fresh}
+  notFull := TensorBank.wf
+  fresh {c} _ := c.next_fresh
+  get_set_eq := by simp_all
+  get_set_ne := by grind
+  get_empty := by simp_all
+  get_hmap := by simp_all
+  get_merge := by simp_all
+  get_fresh {c} H := H _ c.next_fresh.le_refl
+  notFull_empty := by simp
+  notFull_set_fresh {b v} H := by
+    simp <;> intro n Hn
+    split
+    · omega
+    · apply H
+      omega
 
-def DualMemory.get_store {α} (d : DualMemory α) (ix : DualMemoryStoreIndex) (_ : in_memory d ix) :
-    LocalStore α :=
-  match ix with | .in_bounded => d.bounded.toLocalStore | .in_unbounded i => d.unbounded[i]
+instance {α β} : HasHHMap (TensorBank α) (TensorBank β) Nat (LocalStore α) (LocalStore β) where
+  hhmap f s := ⟨fun i => Store.get s i |>.bind (f i), s.next_fresh⟩
+  hhmap_get {t k} f := by simp [Store.get]
 
-/-- A multiaffine equation describing an access into a free coordinate of an Address -/
-structure AffineMap where
-  free_offset : Int
-  free_strides : List Int
-  par_offset : Int
-  par_stride : Int
-  deriving Repr, BEq
+/-- Updating the store preserves wf -/
+theorem TensorBank.set_wf {c : TensorBank α} (Hwf : wf c) : wf (set c n v) := by
+  simp_all [Store.set]
+  intro n' Hn'
+  split <;> rename_i h; omega
+  apply Hwf
+  omega
 
-def AffineMap.par (a : AffineMap) (i : Int) : Int :=
-  a.par_offset + a.par_stride * i
+/-- Hmap over the store preserves wf -/
+theorem TensorBank.hmap_wf {c : TensorBank α} (Hwf : wf c) : wf (hmap f c) := by
+  simp_all [Heap.hmap]
 
-def AffineMap.free (a : AffineMap) (i : List Int) : Int :=
-  a.free_offset + List.dot a.free_strides i
+/-- Merging stores preserves wf -/
+theorem TensorBank.merge_wf {x y : TensorBank α} (Hwfx : wf x) (Hwfy : wf y) : wf (merge op x y) := by
+  simp_all [Heap.merge]
+  intro n Hn
+  rw [Hwfx _ (by omega), Hwfy _ (by omega)]
+  rfl
 
-def AffineMap.is_trivial (a : AffineMap) : Prop :=
-  a.free_offset = 0 ∧
-  a.par_offset = 0 ∧
-  a.par_stride = 1 ∧
-  a.free_strides = a.free_strides.map (fun _ => 1)
+
+/-- Structure describing the physical characteristics of a chip's memory banks -/
+structure ChipMemorySpec where
+  psumPhysSpec : PhyStoreSpec
+  sbufPhysSpec : PhyStoreSpec
 
 structure ChipMemory (α : Type _) where
-  sbuf : DualMemory α
-  psum : DualMemory α
-  hbm : UnboundedBank α
+  psumPhysical  : LocalStore α
+  psumUnbounded : TensorBank α
+  sbufPhysical  : LocalStore α
+  sbufUnbounded : TensorBank α
+  hbmUnbounded  : TensorBank α
+
+inductive ChipIndex
+| psumPhysIndex (index : Nat × Nat)
+| psumUnboundedIndex (tensor : Nat) (index : Nat × Nat)
+| sbufPhysIndex (index : Nat × Nat)
+| sbufUnboundedIndex (tensor : Nat) (index : Nat × Nat)
+| hbmIndex (tensor : Nat) (index : Nat × Nat)
+
+@[simp] def ChipMemory.get (c : ChipMemory α) (i : ChipIndex) : Option α :=
+  match i with
+  | .psumPhysIndex i        => Store.get c.psumPhysical i
+  | .psumUnboundedIndex t i => Store.get c.psumUnbounded t |>.bind (Store.get · i)
+  | .sbufPhysIndex i        => Store.get c.sbufPhysical i
+  | .sbufUnboundedIndex t i => Store.get c.sbufUnbounded t |>.bind (Store.get · i)
+  | .hbmIndex t i           => Store.get c.hbmUnbounded t  |>.bind (Store.get · i)
+
+@[simp] def ChipMemory.set (c : ChipMemory α) (i : ChipIndex) (v : Option α) : ChipMemory α :=
+  match i with
+  | .psumPhysIndex i =>
+      { c with psumPhysical  := Store.set c.psumPhysical i v }
+  | .psumUnboundedIndex t i =>
+      let tgt := Store.get c.psumUnbounded t |>.getD Heap.empty
+      { c with psumUnbounded := Store.set c.psumUnbounded t <| some <| Store.set tgt i v }
+  | .sbufPhysIndex i =>
+      { c with sbufPhysical  := Store.set c.sbufPhysical i v }
+  | .sbufUnboundedIndex t i =>
+      let tgt := Store.get c.sbufUnbounded t |>.getD Heap.empty
+      { c with sbufUnbounded := Store.set c.sbufUnbounded t <| some <| Store.set tgt i v }
+  | .hbmIndex t i =>
+      let tgt := Store.get c.hbmUnbounded t |>.getD Heap.empty
+      { c with hbmUnbounded := Store.set c.hbmUnbounded t <| some <| Store.set tgt i v }
+
+@[simp] def ChipMemory.empty : ChipMemory α := ⟨Heap.empty, Heap.empty, Heap.empty, Heap.empty, Heap.empty⟩
+
+@[simp] def ChipMemory.hmap (f : ChipIndex → α → Option α) (t : ChipMemory α) : ChipMemory α :=
+  ⟨ Heap.hmap (f <| .psumPhysIndex ·) t.psumPhysical,
+    Heap.hmap (fun store_i store_v => some <| Heap.hmap (fun i v => f (.psumUnboundedIndex store_i i) v) store_v) t.psumUnbounded,
+    Heap.hmap (f <| .sbufPhysIndex ·) t.sbufPhysical,
+    Heap.hmap (fun store_i store_v => some <| Heap.hmap (fun i v => f (.sbufUnboundedIndex store_i i) v) store_v) t.sbufUnbounded,
+    Heap.hmap (fun store_i store_v => some <| Heap.hmap (fun i v => f (.hbmIndex store_i i) v) store_v) t.hbmUnbounded ⟩
+
+@[simp] def ChipMemory.merge (op : α → α → α) (x y : ChipMemory α) : ChipMemory α :=
+  ⟨ Heap.merge op x.psumPhysical y.psumPhysical,
+    Heap.merge (Heap.merge op) x.psumUnbounded y.psumUnbounded,
+    Heap.merge op x.sbufPhysical y.sbufPhysical,
+    Heap.merge (Heap.merge op) x.sbufUnbounded y.sbufUnbounded,
+    Heap.merge (Heap.merge op) x.hbmUnbounded y.hbmUnbounded ⟩
+
+theorem ChipMemory.get_set_eq {t : ChipMemory α} {k k' : ChipIndex} {v} : k = k' → get (set t k v) k' = v := by
+  intro H; cases k' <;> simp_all [Store.get_set_eq]
+
+theorem ChipMemory.get_set_ne {t : ChipMemory α} {k k' : ChipIndex} {v} : k ≠ k' → get (set t k v) k' = get t k' := by
+  intro H
+  cases k <;> cases k' <;> simp only [get, set]
+  · rw [Store.get_set_ne (H <| congrArg ChipIndex.psumPhysIndex ·)]
+  · sorry
+  · rw [Store.get_set_ne (H <| congrArg ChipIndex.sbufPhysIndex ·)]
+  · sorry
+  · sorry
+
+theorem ChipMemory.get_empty : get (empty : ChipMemory α) k = none := by
+  cases k <;> simp [empty, Heap.get_empty]
+
+theorem ChipMemory.get_hmap : get (hmap f t) k = (get t k).bind (f k) := by
+  cases k
+  · simp [hmap, Heap.get_hmap]
+  · simp only [get, hmap]
+    sorry
+  · simp [hmap, Heap.get_hmap]
+  · sorry
+  · sorry
+
+theorem ChipMemory.get_merge : get (merge op t1 t2) k = Option.merge op (get t1 k) (get t2 k) := by
+  cases k
+  · simp [hmap, Heap.get_merge]
+  · sorry
+  · simp [hmap, Heap.get_merge]
+  · sorry
+  · sorry
+
+instance ChipMemoryHeapInst : Heap (ChipMemory α) ChipIndex α where
+  get        := ChipMemory.get
+  set        := ChipMemory.set
+  empty      := ChipMemory.empty
+  hmap       := ChipMemory.hmap
+  merge      := ChipMemory.merge
+  get_set_eq := ChipMemory.get_set_eq
+  get_set_ne := ChipMemory.get_set_ne
+  get_empty  := ChipMemory.get_empty
+  get_hmap   := ChipMemory.get_hmap
+  get_merge  := ChipMemory.get_merge
+
+instance {α β} : HasHHMap (ChipMemory α) (ChipMemory β) ChipIndex α β where
+  hhmap f h :=
+    ⟨ hhmap (fun i => f (.psumPhysIndex i)) h.psumPhysical,
+      hhmap (fun i i_store => some <| hhmap (fun j => f (.psumUnboundedIndex i j)) i_store) h.psumUnbounded,
+      hhmap (fun i => f (.psumPhysIndex i)) h.sbufPhysical,
+      hhmap (fun i i_store => some <| hhmap (fun j => f (.sbufUnboundedIndex i j)) i_store) h.sbufUnbounded,
+      hhmap (fun i i_store => some <| hhmap (fun j => f (.hbmIndex i j)) i_store) h.hbmUnbounded ⟩
+  hhmap_get {t k} f := by
+    cases k <;> simp_all [Store.get]
+    · sorry
+    · sorry
+    · sorry
+    · sorry
+    · sorry
+
+structure ProdStore (T : Type _) where
+  left  : T
+  right : T
+
+inductive ProdIndex (K : Type _) where
+| left  (k : K)
+| right (k : K)
+
+instance [Heap T K V] : Heap (ProdStore T) (ProdIndex K) V where
+  get h k :=
+    match k with
+    | .left k => Store.get h.left k
+    | .right k => Store.get h.right k
+  set h k v :=
+    match k with
+    | .left k => { h with left := Store.set h.left k v }
+    | .right k => { h with right := Store.set h.right k v }
+  empty := ⟨ Heap.empty, Heap.empty ⟩
+  hmap f h := ⟨ Heap.hmap (fun k v => f (.left k)  v) h.left, Heap.hmap (fun k v => f (.right k) v) h.right ⟩
+  merge op x y := ⟨ Heap.merge op x.left y.left, Heap.merge op x.right y.right ⟩
+  get_set_eq {t k k' v} H := by cases k' <;> cases k <;> simp_all [Store.get_set_eq]
+  get_set_ne {t k k' v} H := by cases k' <;> cases k <;> simp_all [Store.get_set_ne]
+  get_empty {k} := by cases k <;> simp_all [Heap.get_empty]
+  get_hmap {f t k} := by cases k <;> simp_all [Heap.get_hmap]
+  get_merge {op x y} k := by cases k <;> simp_all [Heap.get_merge]
+
+
+instance [Heap T1 K V1] [Heap T2 K V2] [HasHHMap T1 T2 K V1 V2] :
+    HasHHMap (ProdStore T1) (ProdStore T2) (ProdIndex K) V1 V2 where
+  hhmap f h := ⟨ hhmap (fun i v => f (.left i) v) h.1,  hhmap (fun i v => f (.right i) v) h.2⟩
+  hhmap_get {t k} f := by cases k <;> simp [hhmap_get, Store.get]
 
 /-- The memory that can be stored in a UnboundedStore -/
 inductive UCell (α DataT : Type _)
@@ -111,38 +300,13 @@ inductive UCell (α DataT : Type _)
 | Data (_ : DataT)
 
 abbrev NeuronMemory (DataT : Type _) := ChipMemory (UCell UInt8 DataT)
+abbrev NeuronIndex := ChipIndex
 
+abbrev ProdNeuronMemory (DataT : Type _) := ProdStore (ChipMemory (UCell UInt8 DataT))
+abbrev ProdNeuronIndex := ProdIndex ChipIndex
 
-structure ProdChipMemory (T : Type _) where
-  left : KLR.Core.ChipMemory T
-  right : KLR.Core.ChipMemory T
-
-inductive ProdIndex
-| left (_ : KLR.Core.DualMemoryStoreIndex)
-| right (_ : KLR.Core.DualMemoryStoreIndex)
-
-section iris
--- TODO: Stabilize Heap in Iris-Lean
-instance {T : Type _} : AllocHeap (ProdChipMemory T) ProdIndex T where
-  get := sorry
-  set := sorry
-  fresh := sorry
-  get_set_eq := sorry
-  get_set_ne := sorry
-  empty := sorry
-  hmap := sorry
-  merge := sorry
-  get_empty := sorry
-  get_hmap := sorry
-  get_merge := sorry
-  notFull := sorry
-  get_fresh := sorry
-
-
+/-
 instance {T1 T2 : Type _} : HasHHMap (ProdChipMemory T1) (ProdChipMemory T2) ProdIndex T1 T2 where
   hhmap := sorry
   hhmap_get := sorry
-
-end iris
-
--- def TProd (H : Type _ → Type _) (T : Type _) : Type _ := H T × H T
+-/
